ğŸ‘ˆ [[1 æé™ä¸è¿ç»­æ€§]]

## åŸºæœ¬åˆç­‰å‡½æ•°çš„å¯¼æ•°

$$(\tan x)^\prime = \sec^2 x$$
$$(\cot x)^\prime = - \csc^2 x$$
$$(\sec x)^\prime = \sec x \tan x$$
$$(\csc x)^\prime = - \csc x \cot x$$
$$(\arcsin x)^\prime = \frac{1}{\sqrt{1 - x^2}}$$
$$(\arccos x)^\prime = - \frac{1}{\sqrt{1 - x^2}}$$
$$(\arctan x)^\prime = \frac{1}{1 + x^2}$$
$$({\rm{arccot}} x)^\prime = - \frac{1}{1 + x^2}$$

## é«˜é˜¶å¯¼æ•°

è±å¸ƒå°¼èŒ¨å…¬å¼ï¼ˆè¿ç®—æ³•åˆ™ï¼Œç±»ä¼¼äºäºŒé¡¹å¼å±•å¼€ï¼‰ï¼š

$$(uv)^{(n)} = \sum_{k = 0}^n C_n^k u^{(k)} v^{(n - k)}$$

å¸¸ç”¨å‡½æ•°çš„é«˜é˜¶å¯¼æ•°ï¼š

$$({\rm e}^{a x + b})^{(n)} = a^n {\rm e}^{(a x + b)}$$
$$(\sin{(a x + b)})^{(n)} = a^n \sin{(a x + b + \frac{n \pi}{2})}$$
$$(\cos{(a x + b)})^{(n)} = a^n \cos{(a x + b + \frac{n \pi}{2})}$$
$$(\frac{1}{a x + b})^{(n)} = \frac{(-1)^n n! a^n}{(a x + b)^{n + 1}}$$

## éšå‡½æ•°æ±‚å¯¼

### å¹‚æŒ‡å‡½æ•°æ±‚å¯¼

å¯¹$y = u(x)^{v(x)}$ï¼Œä¸¤è¾¹å–å¯¹æ•°å˜ä¸º$\ln{y} = v(x) \ln{u(x)}$ï¼Œæˆ–å˜ä¸º$y = e^{v(x) \ln{u(x)}}$ï¼Œå†æ±‚å¯¼ã€‚

## å¾®åˆ†

å¯å¾®$\iff$å¯å¯¼$\implies$è¿ç»­

### è¿‘ä¼¼è®¡ç®—

$x \to x_0$æ—¶ï¼Œ$f(x) \approx f(x_0) + f^\prime (x_0) (x - x_0)$

ğŸ‘‰ [[3 å¾®åˆ†ä¸­å€¼å®šç†ä¸å¯¼æ•°çš„åº”ç”¨]]